@prefix owl: <http://www.w3.org/2002/07/owl#> .
@prefix xsd: <http://www.w3.org/2001/XMLSchema#> .
@prefix geo: <http://www.w3.org/2003/01/geo/wgs84_pos#> .
@prefix rdfs: <http://www.w3.org/2000/01/rdf-schema#> .
@prefix rdf: <http://www.w3.org/1999/02/22-rdf-syntax-ns#> .
@prefix tA: <http://www.example.com/touristAsist#> .


#Class definitions

tA:Country 				rdf:type				owl:Class;
						rdfs:comment 			"A country of interest for user" .

tA:Locality 			rdf:type				owl:Class;
						geo:lat					xsd:double ;
						geo:long 				xsd:double ;
						rdfs:comment			"A locality of interest for user" .

tA:Destination 			rdf:type                owl:Class ;
						rdfs:subClassOf         tA:Locality ;
						rdfs:comment            "The main point of interest in an itinerary" .

tA:Accomodation 		rdf:type 				owl:Class ;
						geo:lat					xsd:double ;
						geo:long 				xsd:double ;
						rdfs:comment     		"A place where a person can sleep" .

tA:Restaurant			rdf:type 				owl:Class ;
						geo:lat					xsd:double ;
						geo:long 				xsd:double ;
						rdfs:comment			"A place where a person can have breakfast/dinner/lunch" .

tA:TouristicObjective   rdf:type 				owl:Class ;
						geo:lat					xsd:double ;
						geo:long 				xsd:double ;
						rdfs:comment			"A touristic objective of interest" .

tA:NaturalAttraction    rdf:type				owl:Class ;
						rdfs:subClassOf         tA:TouristicObjective ;
						rdfs:comment 			"A mountain, lake, seaside, forest or something related activities in nature" .

tA:CulturalAttraction   rdf:type     			owl:Class ;
						rdfs:subClassOf         tA:TouristicObjective ;
						rdfs:comment      		"A a theatre, museum or something related to cultural acitvities" .

tA:Museum 				rdf:type				owl:Class ;
						rdfs:subClassOf         tA:CulturalAttraction ;
						rdfs:comment			"Museum" .

tA:Theatre 				rdf:type 				owl:Class ;
						rdfs:subClassOf 		tA:CulturalAttraction ;  
						rdfs:comment            "Theatre" .

tA:OtherCulturalAttraction rdf:type  			owl:Class ;
						   rdfs:subClassOf      tA:CulturalAttraction ;
						   rdfs:comment 		"Other cultural attraction of interest" .

tA:Mountain 			rdf:type 				owl:Class ;
						rdfs:subClassOf 		tA:NaturalAttraction ;
						rdfs:comment            "A mountain peak or region".

tA:Seaside 				rdf:type 				owl:Class;
						rdfs:subClassOf 		tA:NaturalAttraction ;
						rdfs:comment 			"A region with sea, oceans etc" .	

tA:Lake 				rdf:type				owl:Class ;
						rdfs:subClassOf 		tA:NaturalAttraction ;
						rdfs:comment 			"Lake " .


tA:OtherNaturalAttraction rdf:type   			owl:Class ;
						  rdfs:subClassOf 		tA:NaturalAttraction ;
						  rdfs:comment			"Other natural attractions (batai cu ursul)". 


tA:Activity 			rdf:type 				owl:Class ;
						rdfs:comment 			"An activity which ca be held at a Place" .

tA:CulturalActivity 	  rdf:type 				owl:Class ;
						  rdfs:subClassOf 		tA:Activity ;
						  rdfs:comment 			"An activity held at a cultural touristic objective" .

tA:EntertainmentActivity 	  rdf:type 				owl:Class ;
						      rdfs:subClassOf 		tA:Activity ;
						      rdfs:comment 			"An activity preffered by a tourist who wants to relax" .						  

tA:AdventureActivity 	  rdf:type 				owl:Class ;
						  rdfs:subClassOf 		tA:Activity ;
						  rdfs:comment 			"An activity held at a natural touristic objective" .

tA:Itinerary 			  rdf:type 				owl:Class;
						  rdfs:comment			"A full itinerary planned by a user" .	

tA:FamilyItinerary		  rdf:type 				owl:Class;
						  rdfs:subClassOf       tA:Itinerary ;
						  rdfs:comment 			"An itinerary suitable for a family with kids".

tA:AdventureItinerary     rdf:type				owl:Class;
						  rdfs:subClassOf		tA:Itinerary ;
						  rdfs:comment   		"An itinerary suitable for a single person ".


#Properties

tA:name 					rdf:type 			owl:DatatypeProperty ;
							rdfs:domain         tA:Restaurant, tA:Accomodation, tA:TouristicObjective, tA:Activity, tA:Locality, tA:Country ;
							rdfs:range    		xsd:string ;
							rdfs:comment        "Name of the resource".		

tA:description				rdf:type 			owl:DatatypeProperty ;
							rdfs:domain 		tA:Restaurant, tA:Accomodation, tA:TouristicObjective, tA:Activity, tA:Country, tA:Locality, tA:Itinerary ;
							rdfs:range 			xsd:string ;
 							rdfs:comment 		"Description of an entity" .

tA:include					rdf:type 			owl:ObjectProperty ;
							rdfs:domain 		tA:Country;
							rdfs:range			tA:Locality;
							rdfs:comment		"A country contains many localities".

tA:isIncludedBy				rdf:type 			owl:ObjectProperty ;
							rdfs:range 			tA:Country;
							rdfs:domain			tA:Locality;
							owl:inverseOf       tA:include; 
							rdfs:comment		"A country contains many localities".


tA:isNearBy 				rdf:type 			owl:ObjectProperty ;
							rdfs:domain	 		tA:Locality;
							rdfs:range  		tA:Restaurant,tA:Accomodation,tA:TouristicObjective;
							rdfs:comment 		"A locality is near an entity if the distance is bigger than 10 km and smaller than 30 km".

tA:inProximity				rdf:type 			owl:ObjectProperty ;
							rdfs:domain         tA:Restaurant,tA:Accomodation,tA:TouristicObjective;
							rdfs:range 			tA:Locality;
							owl:inverseOf       tA:isNearBy; 
							rdfs:comment		"An entity isin proximity of a locality if the distance is bigger than 10 km smaller than 30km".

tA:contains 				rdf:type 			owl:ObjectProperty ;
							rdfs:domain	 		tA:Locality;
							rdfs:range  		tA:Restaurant,tA:Accomodation,tA:TouristicObjective;
							rdfs:comment 		"A locality contains an entity if the distance is smaller than 10 km".

tA:isContainedBy			rdf:type 			owl:ObjectProperty ;
							rdfs:domain         tA:Restaurant,tA:Accomodation,tA:TouristicObjective;
							rdfs:range 			tA:Locality;
							owl:inverseOf       tA:isNearBy; 
							rdfs:comment		"An entity is in contained by locality if the distance is smaller than 10 km ".

tA:isSpecificTo    			rdf:type 			owl:ObjectProperty ;
							rdfs:domain 		tA:CulturalActivity,tA:EntertainmentActivity ;
							rdfs:range 			tA:CulturalAttraction ;
							rdfs:comment 		"A cultural activity can be held in proximity of a cultural attraction".

tA:isHeldAt					rdf:type			owl:ObjectProperty ;
							rdfs:domain			tA:AdventureActivity, tA:EntertainmentActivity ;
							rdfs:range			tA:NaturalAttraction ;
							rdfs:comment		"An adventure activity is held in proximity of a natural attraction".

tA:embracedBy				rdf:type 			owl:ObjectProperty ;
							rdfs:domain 		tA:CulturalActivity,tA:EntertainmentActivity ;
							rdfs:range 			tA:FamilyItinerary ;
							rdfs:comment 		"Activities preffered in a Family Itinerary" .

tA:preferredBy				rdf:type			owl:ObjectProperty ;
							rdfs:domain 		tA:AdventureActivity, tA:EntertainmentActivity ;
							rdfs:range 			tA:AdventureItinerary ;
							rdfs:comment		"Activities preffered by a single person who wants to have fun".


tA:hasScheduled				rdf:type			owl:ObjectProperty ;
							rdfs:domain			tA:Itinerary;
							rdfs:range			tA:Destination;
							rdfs:comment		"Each itinerary will have a main destination".

tA:wasScheduledFor			rdf:type			owl:ObjectProperty ;
							rdfs:domain			tA:Destination;
							rdfs:range			tA:Itinerary;
							rdfs:comment		"Each Destination is scheduled for an itinerary".

tA:isSelectedFor			rdf:type			owl:ObjectProperty ;
							rdfs:domain 		tA:Restaurant,tA:Accomodation,tA:TouristicObjective;
							rdfs:range 			tA:Itinerary;
							rdfs:comment		"An entity visited in user defined itinerary".

tA:involve					rdf:type 			owl:ObjectProperty ;
							rdfs:domain			tA:Itinerary;
							rdfs:range			tA:Restaurant,tA:Accomodation,tA:TouristicObjective;
							owl:inverseOf       tA:isSelectedFor; 
							rdfs:comment		"An itinerary has touristic objectives, food places and hotels".

tA:hasCapital				rdf:type			owl:ObjectProperty;
							rdfs:domain			tA:Country;
							rdfs:range			tA:Locality;
							rdfs:comment		"Every country has a capital".

tA:isCapitalOf				rdf:type			owl:ObjectProperty;
							rdfs:domain			tA:Locality;
							rdfs:range 			tA:Country;
							owl:inverseOf       tA:hasCapital;
							rdfs:comment		"A locality can be the capital of a country". 



